regexp/compilation/regexpExampleVerilogPrintLib.sml
@@ -1,0 +1,64 @@
+open regexpExampleVerilogTheory;
+
+open verilogTranslatorConfigLib verilogTranslatorCoreLib verilogTranslatorLib verilogPrintLib;
+
+open verilogSyntax;
+
+val ERR = Feedback.mk_HOL_ERR "regexpExampleVerilogPrintLib";
+
+(* test: circuit_correct_regexp_verilog *)
+
+(* verilog code: *)
+regexpv_def |> concl |> rhs |> vprog_print |> print
+
+(* variables: *)
+``var_type_print relMtypes`` |> EVAL
+
+(*
+
+We do not treat initialization formally,
+but given how this code looks like we probably should:
+
+fun vectorToList vec = Vector.foldr (op ::) [] vec;
+fun toVerilogList l =
+ l
+ |> rev
+ |> String.concatWith ", "
+ |> (fn l => "'{" ^ l ^ "}");
+
+fun toVerilogListInit name l =
+ l
+ |> mapi (fn i => fn e => name ^ "[" ^ (Int.toString i) ^ "] = " ^ e);
+
+ regexp_res
+ |> #final
+ |> vectorToList
+ |> rev
+ |> map (fn b => if b then "1" else "0")
+ |> String.concatWith ", "
+ |> (fn bs => "'{" ^ bs ^ "}")
+
+ regexp_res
+ |> #table
+ |> vectorToList
+ |> map vectorToList
+ |> map (map Int.toString)
+ |> map toVerilogList
+ |> toVerilogListInit "next_state_info"
+ |> String.concatWith ";\n"
+ |> print
+ 
+ regexp_res
+ |> #table
+ |> vectorToList
+ |> tl
+ |> tl
+ |> hd
+ |> vectorToList
+ |> el 112
+
+state_size
+hfinal
+htable
+
+*)
