translator/verilogLiftLib.sml
@@ -11,32 +11,33 @@ open verilogSyntax;
 
 local
 val (var_has_type_tm, mk_var_has_type, dest_var_has_type, is_var_has_type) = syntax_fns3 "verilogType" "var_has_type";
+
+fun thm_pred th = th |> SPEC_ALL |> concl |> lhs |> rand
+
+val conv_thms =
+ [var_has_type_old_var_has_type_BOOL,
+  var_has_type_old_var_has_type_WORD,
+  var_has_type_old_var_has_type_WORD_ARRAY_BOOL,
+  var_has_type_old_var_has_type_WORD_ARRAY,
+  var_has_type_old_var_has_type_WORD_ARRAY_WORD_ARRAY]
+ |> map (fn th => (thm_pred th, th));
+
+fun lookup_match_term x nil = failwith "unknown verilog type"
+  | lookup_match_term x ((k, v) :: ls) = if can (match_term k) x then v else lookup_match_term x ls;
 in
 fun var_has_type_to_old_CONV tm =
  if is_abs tm then
    ABS_CONV var_has_type_to_old_CONV tm
  else if is_var_has_type tm then let
-   val (_, _, ty) = dest_var_has_type tm
+   val (_, var, ty) = dest_var_has_type tm
+   val pred = var |> fromHOLstring |> predicate_for_var
+   (* inefficient but works: *)
+   val pred_thm = lookup_match_term pred conv_thms
+   val pred_thm = PART_MATCH (rand o lhs) pred_thm pred
+                  |> CONV_RULE (RHS_CONV (RAND_CONV EVAL))
+                  |> SYM
  in
-   if is_VBool_t ty then (* BOOL *)
-     PURE_REWRITE_CONV [GSYM var_has_type_old_var_has_type_BOOL] tm
-   else if is_VArray_t ty then let
-     val is = dest_VArray_t ty
-     val len = length is
-   in
-     if len = 1 then (* WORD, TODO: assumes numerals in index position *) let
-       val dimindex_rw = is |> hd |> dest_numeral |> mk_numeric_type |> mk_dimindex |> EVAL |> SYM
-     in
-       PURE_REWRITE_CONV [dimindex_rw, GSYM var_has_type_old_var_has_type_WORD] tm
-     end else if len = 2 then (* WORD_ARRAY, TODO: does not work if index same... *) let
-       val dimword_rw = is |> hd |> dest_numeral |> Arbnumcore.log2 |> mk_numeric_type |> mk_dimword |> EVAL |> SYM
-       val dimindex_rw = is |> tl |> hd |> dest_numeral |> mk_numeric_type |> mk_dimindex |> EVAL |> SYM
-     in
-       PURE_REWRITE_CONV [dimword_rw, dimindex_rw, GSYM var_has_type_old_var_has_type_WORD_ARRAY] tm
-     end else
-       ALL_CONV tm
-   end else
-     ALL_CONV tm
+  PURE_REWRITE_CONV [pred_thm] tm
  end else if is_comb tm then
    COMB_CONV var_has_type_to_old_CONV tm
  else ALL_CONV tm
