regexp/compilation/regexpExampleVerilogScript.sml
@@ -1,0 +1,99 @@
+open hardwarePreamble;
+
+open verilogTranslatorLib moduleTranslatorTheory;
+open verilogTranslatorConfigLib verilogLiftLib;
+
+open regexpExampleTheory;
+
+val _ = new_theory "regexpExampleVerilog";
+
+val _ = guess_lengths ();
+val _ = prefer_num ();
+
+(* Main process *)
+val trans = hol2hardware_step_function regexp_def;
+val prog_def = EvalS_get_prog (trans |> concl);
+val regexpv_def = Define `regexpv = ^prog_def`;
+val trans = REWRITE_RULE [GSYM regexpv_def] trans;
+
+(* Ad-hoc lifting as we only have one process and no non-blocking writes *)
+val regexp_step_relM = Q.store_thm("regexp_step_relM",
+ `!n fext fextv init vs ps.
+  (* Simulation step *)
+  relM (circuit init fext n) vs /\ lift_fext fextv fext
+  ==>
+  ?vs'. mstep_commit (fextv n) [regexpv] vs = INR vs' /\
+        relM (circuit init fext (SUC n)) vs'`,
+ rewrite_tac [lift_fext_relS_fextv_fext] \\
+ rw [mstep_commit_def, mstep_def, sum_foldM_def] \\
+ first_x_assum (qspec_then `n` assume_tac) \\
+ drule_strip relM_relS \\
+ drule_strip (trans |> REWRITE_RULE [EvalS_def] |> GEN_ALL) \\
+
+ drule vnwrites_nil_correct \\ impl_tac >- EVAL_TAC \\ strip_tac \\
+ fs [sum_bind_def, sum_map_def, circuit_def] \\
+ fs [relS_def, relM_def, relS_var_def, relM_var_def, mget_var_get_var]);
+
+val regexp_step_relM_run = Q.store_thm("regexp_step_relM_run",
+ `!n fextv fext init vs.
+  relM init vs /\ lift_fext fextv fext
+  ==>
+  ?vs'. mrun fextv [regexpv] vs n = INR vs' /\
+        relM (circuit init fext n) vs'`,
+ rpt strip_tac \\ match_mp_tac mstep_commit_mrun \\ qexists_tac `[]` \\ rpt conj_tac
+ >- simp [circuit_def]
+ >- simp [vars_has_type_def]
+ \\ rpt strip_tac \\ match_mp_tac regexp_step_relM \\ simp []);
+
+(* circuit_correct_regexp *)
+
+val INIT_verilog_def = Define `
+ INIT_verilog env <=>
+  (* Machine implementation registers *)
+  WORD (0w:word4) (THE (ALOOKUP env "state")) /\
+  WORD (0w:word4) (THE (ALOOKUP env "state_start")) /\
+
+  WORD_ARRAY BOOL (hwfinal : word4 -> bool) (THE (ALOOKUP env "state_is_final")) /\
+  (WORD_ARRAY (WORD_ARRAY WORD)) (hwtable : word4 -> word8 -> word4) (THE (ALOOKUP env "next_state_info"))`;
+
+val relM_backwards = Q.store_thm("relM_backwards",
+ `!vs. vars_has_type vs relMtypes ==> ?hol_s. relM hol_s vs`,
+ simp [vars_has_type_def, relMtypes_def, relM_def, relM_var_def, mget_var_ALOOKUP] \\ rpt gen_tac \\
+
+ relM_backwards_tac);
+
+val INIT_backwards = Q.store_thm("INIT_backwards",
+ `!hol_s init.
+   relM hol_s init /\
+   INIT_verilog init ==>
+   INIT hol_s`,
+ rw [INIT_verilog_def, relM_def, relM_var_def, mget_var_def] \\
+ every_case_tac \\ fs [] \\ rveq \\
+ simp [INIT_def] \\
+ metis_tac [WORD_eq, WORD_ARRAY_BOOL_eq, WORD_ARRAY_WORD_ARRAY_WORD_eq]);
+
+val circuit_correct_regexp_verilog = Q.store_thm("circuit_correct_regexp_verilog",
+ `!n m init fext fextv.
+  lift_fext fextv fext /\
+
+  vars_has_type init relMtypes /\
+  INIT_verilog init /\
+
+  (fext n).new_package /\
+  (∀p. p ≤ m ⇒ ¬(fext (n + p)).new_package)
+  ==>
+  ?vs'.
+   mrun fextv [regexpv] init (SUC (n + m)) = INR vs' /\
+   mget_var vs' "accept" = INR (VBool (regexp_lang foobar_regex (str_of_ext fext (n + 1) m)))`,
+ rpt strip_tac \\
+ drule_strip relM_backwards \\
+ drule_strip INIT_backwards \\
+ drule_strip regexp_step_relM_run \\
+ first_x_assum (qspec_then `SUC (n + m)` strip_assume_tac) \\
+ simp [] \\
+
+ fs [relM_def, relM_var_def, BOOL_def] \\
+ drule_strip circuit_correct_regexp \\
+ fs []);
+
+val _ = export_theory ();
