regexp/regexpExampleScript.sml
@@ -1,0 +1,449 @@
+open hardwarePreamble;
+
+open arithmeticTheory stringTheory;
+
+open dep_rewrite;
+
+open regexp_compilerTheory;
+
+val _ = new_theory "regexpExample";
+
+val _ = guess_lengths ();
+val _ = prefer_num ();
+
+(****
+ Cleaner DFA semantics
+ ****)
+
+(* exec_dfa, but also return last state, and Vector + option wrappers *)
+val exec_dfa_state_def = Define `
+ (exec_dfa_state finals table n "" = (EL n finals, n)) /\
+ (exec_dfa_state finals table n (STRING c t) =
+  exec_dfa_state finals table (EL (ORD c) (EL n table)) t)`;
+
+(*val exec_dfa_state_ind = theorem "exec_dfa_state_ind";*)
+
+(*
+val cleanup_finals_def = Define `
+ cleanup_finals (Vector fs) = fs`;
+
+val cleanup_Vectors_def = Define `
+ (cleanup_Vectors [] = []) /\
+ (cleanup_Vectors (Vector x::xs) = x :: cleanup_Vectors xs)`;
+
+val cleanup_SOMEs_def = Define `
+ (cleanup_SOMEs [] = SOME []) /\
+ (cleanup_SOMEs (NONE :: xs) = NONE) /\
+ (cleanup_SOMEs (SOME x :: xs) = case cleanup_SOMEs xs of
+                                     SOME xs => SOME (x :: xs)
+                                   | NONE => NONE)`;
+
+val cleanup_table_def = Define `
+ cleanup_table (Vector table) = cleanup_SOMEs (MAP cleanup_SOMEs (cleanup_Vectors table))`;
+
+val cleanup_Vectors_MAP_Vector = Q.store_thm("cleanup_Vectors_MAP_Vector",
+ `!xs. cleanup_Vectors (MAP Vector xs) = xs`,
+ Induct \\ rw [cleanup_Vectors_def]);
+*)
+
+val from_hfinals_def = Define `
+ from_hfinals = Vector`;
+
+val from_htable_def = Define `
+ from_htable = Vector o (MAP (Vector o MAP SOME))`;
+
+val exec_dfa_state_APPEND = Q.store_thm("exec_dfa_state_APPEND",
+ `!str1 str2 finals table n n' accept.
+   exec_dfa_state finals table n str1 = (accept, n') /\ str2 <> "" ==>
+   exec_dfa_state finals table n (APPEND str1 str2) = exec_dfa_state finals table n' str2`,
+ Induct \\ rpt strip_tac \\ fs [exec_dfa_state_def]);
+
+(****
+ Regexp example
+ ****)
+
+val regexp = Regexp_Type.fromString "fo+bar";
+val regexp_res = regexpLib.matcher regexpLib.HOL regexp;
+
+val cert = #certificate regexp_res |> valOf;
+
+local
+ val regexp_term = cert |> SPEC_ALL |> concl |> rhs |> rator |> rand
+in
+val foobar_regex_def = Define `
+ foobar_regex = ^regexp_term`;
+end;
+
+val cert = cert |> REWRITE_RULE [GSYM foobar_regex_def];
+
+fun mk_list' l ty =
+ Vector.foldr listSyntax.mk_cons (listSyntax.mk_nil ty) l;
+
+fun mk_bool b =
+ if b then T else F;
+
+val hfinal =
+ regexp_res
+ |> #final
+ |> Vector.map mk_bool
+ |> flip mk_list' bool;
+
+val htable =
+ regexp_res
+ |> #table
+ |> Vector.map (flip mk_list' num o Vector.map term_of_int)
+ |> flip mk_list' (listSyntax.mk_list_type num);
+
+val valid_state_def = Define `
+ valid_state nos n <=> n < nos`;
+
+val valid_trans_def = Define `
+ valid_trans nos trans <=>
+  LENGTH trans = nos /\
+  !s. valid_state nos s ==> LENGTH (EL s trans) = 256 /\
+                            (!c. valid_state nos (EL (ORD c) (EL s trans)))`;
+
+val sub_sub_from_clean_table = Q.store_thm("sub_sub_from_clean_table",
+ `!nos trans n m.
+   valid_trans nos trans /\ valid_state nos n ==>
+   sub (sub (from_htable trans) n) (ORD m) = SOME (EL (ORD m) (EL n trans))`,
+ rw [valid_state_def, valid_trans_def, from_htable_def, sub_def, combinTheory.o_DEF,
+     EL_MAP, ORD_BOUND]);
+
+val valid_state_trans = Q.store_thm("valid_state_trans",
+ `!state nos trans n.
+   valid_state nos state /\ valid_trans nos trans ==> valid_state nos (EL (ORD n) (EL state trans))`,
+ rw [valid_trans_def]);
+
+(* Depends on valid trans and state, so place here... *)
+val exec_dfa_state_correct = Q.store_thm("exec_dfa_state_correct",
+ `!s nos finals table n.
+   valid_trans nos table /\ valid_state nos n ==>
+   FST (exec_dfa_state finals table n s) =
+   exec_dfa (from_hfinals finals) (from_htable table) n s`,
+ Induct \\ rpt strip_tac \\ once_rewrite_tac [exec_dfa_state_def, exec_dfa_def]
+ >- simp [from_hfinals_def, sub_def] \\
+ drule_strip sub_sub_from_clean_table \\
+ simp [] \\ drule_strip valid_state_trans \\
+ pop_assum (qspec_then `h` assume_tac) \\
+ first_x_assum drule_strip \\ simp []);
+
+val exec_dfa_state_correct_valid_state_lem = Q.prove(
+ `!s nos finals table n.
+   valid_trans nos table /\ valid_state nos n ==>
+   valid_state nos (SND (exec_dfa_state finals table n s))`,
+ Induct \\ rw [exec_dfa_state_def, valid_trans_def]);
+
+val exec_dfa_state_correct_valid_state = Q.store_thm("exec_dfa_state_correct_valid_state",
+ `!s nos finals table n accept n'.
+   valid_trans nos table /\
+   valid_state nos n /\
+   exec_dfa_state finals table n s = (accept, n') ==>
+   valid_state nos n'`,
+ rpt strip_tac \\ drule_strip exec_dfa_state_correct_valid_state_lem \\
+ pop_assum (qspecl_then [`s`, `finals`] mp_tac) \\ simp []);
+
+(****
+ Circuit
+ ****)
+
+(* Can we just use alpha here instead? *)
+val state_ty = ``:word4``;
+val state_size_ty = wordsSyntax.dest_word_type state_ty;
+val state_size = state_size_ty |> fcpSyntax.dest_numeric_type |> Arbnumcore.toInt;
+(*val state_num_ty =
+ Arbnumcore.pow (Arbnumcore.two, state_size)
+ |> fcpSyntax.mk_numeric_type
+ |> wordsSyntax.mk_word_type;
+val state_size = state_size |> Arbnumcore.toInt;*)
+
+val _ = Datatype `
+ rc = <| (* IO *)
+         accept : bool;
+
+         (* Internal state *)
+         state : ^state_ty;
+         state_start : ^state_ty;
+         state_is_final : ^state_ty -> bool;
+
+         next_state_info : ^state_ty -> word8 -> ^state_ty; (* state -> (char -> state) *)
+       |>`;
+
+val _ = Datatype `
+ rc_ext = <| new_package : bool; data_valid : bool; data : word8 |>`;
+
+val regexp_def = Define `
+ regexp fext (s:rc) =
+  let s' = (if fext.new_package then
+             s with state := s.state_start
+            else if fext.data_valid then
+             s with state := s.next_state_info s.state fext.data
+            else
+             s) in
+  s' with <| accept := s'.state_is_final s'.state |>`; (* reject (= ~accept) ignored for now *)
+
+val regexp_alt = Q.store_thm("regexp_alt",
+ `!fext s. regexp fext s =
+  let s' = (if fext.new_package then
+             s with state := s.state_start
+            else if fext.data_valid then
+             s with state := s.next_state_info s.state fext.data
+            else
+             s) in
+  s' with <| accept := s.state_is_final s'.state |>`,
+ rw [regexp_def]);
+
+val circuit_def = Define `
+ (circuit init fext 0 = init) /\
+ (circuit init fext (SUC n) = regexp (fext n) (circuit init fext n))`;
+
+(* Operations on fext *)
+
+val genlist_option_def = Define `
+ (genlist_option f 0 = []) /\
+ (genlist_option f (SUC n) = case (f n) of
+                              NONE => genlist_option f n
+                            | SOME f_n => SNOC f_n (genlist_option f n))`;
+
+val str_of_ext_def = Define `
+ str_of_ext ext start len =
+  genlist_option (\i. if (ext (start + i)).data_valid then
+                        SOME (CHR (w2n (ext (start + i)).data))
+                      else
+                        NONE) len`;
+
+val str_of_ext_valid_data = Q.store_thm("str_of_ext_valid_data",
+ `!ext n m.
+   (ext (n + m)).data_valid ==>
+   str_of_ext ext n (SUC m) = SNOC (CHR (w2n (ext (n + m)).data)) (str_of_ext ext n m)`,
+ rw [str_of_ext_def, genlist_option_def]);
+
+val str_of_ext_not_valid_data = Q.store_thm("str_of_ext_not_valid_data",
+ `!ext n m. ~(ext (n + m)).data_valid ==> (str_of_ext ext n (SUC m)) = (str_of_ext ext n m)`,
+ rw [str_of_ext_def, genlist_option_def]);
+
+(* More data transformations *)
+
+local
+ val hwnos = ``LENGTH ^hfinal`` |> listLib.LENGTH_CONV |> concl |> rhs
+in
+val hwnos_def = Define `
+ hwnos = ^hwnos`;
+end;
+
+(* hardcoded state size: *)
+val hwfinal_def = Define `
+ hwfinal (s:word4) = if w2n s < hwnos then EL (w2n s) ^hfinal else F`;
+
+(* hardcoded state size: *)
+val hwtable_def = Define `
+ hwtable (s:word4) (c:word8) = if w2n s < hwnos then n2w (EL (w2n c) (EL (w2n s) ^htable)) else (0w:word4)`;
+
+val valid_hardware_state_def = Define `
+ valid_hardware_state nos n = (w2n n < nos)`;
+
+val valid_hardware_trans_def = Define `
+ valid_hardware_trans nos (trans : 'a word -> word8 -> 'a word) =
+  !s c. valid_hardware_state nos s ==> valid_hardware_state nos (trans s c)`;
+
+val from_hardware_trans_def = Define `
+  from_hardware_trans nos trans =
+   GENLIST (\state_i. GENLIST (w2n o (trans (n2w state_i)) o n2w) 256) nos`;
+
+val from_hardware_sif_def = Define `
+  from_hardware_sif nos sif = GENLIST (sif o n2w) nos`;
+
+val valid_hardware_state_trans = Q.store_thm("valid_hardware_state_trans",
+ `!nos state trans n.
+   valid_hardware_state nos state /\ valid_hardware_trans nos trans ==> valid_hardware_state nos (trans state n)`,
+ rw [valid_hardware_trans_def]);
+
+val valid_hardware_state_valid_state_w2n = Q.store_thm("valid_hardware_state_valid_state_w2n",
+ `!nos s. valid_hardware_state nos s ==> valid_state nos (w2n s)`,
+ rw [valid_hardware_state_def, valid_state_def] \\ Cases_on `s` \\ fs [WORD_LO] \\
+ Cases_on `nos < dimword (:'a)` \\ fs []);
+
+val valid_state_valid_hardware_state = Q.store_thm("valid_state_valid_hardware_state",
+ `!nos s. valid_state nos s ==> valid_hardware_state nos (n2w s)`,
+ rw [valid_state_def, valid_hardware_state_def] \\
+ qspecl_then [`dimword (:'a)`, `s`] assume_tac (GEN_ALL MOD_LESS_EQ) \\ fs []);
+
+val valid_hardware_trans_valid_trans = Q.store_thm("valid_hardware_trans_valid_trans",
+ `!nos trans.
+   valid_hardware_trans nos trans ==>
+   valid_trans nos (from_hardware_trans nos trans)`,
+ once_rewrite_tac [valid_trans_def, from_hardware_trans_def] \\ rpt strip_tac
+ >- (once_rewrite_tac [from_hardware_trans_def] \\ simp [])
+ >- (once_rewrite_tac [from_hardware_trans_def] \\ DEP_REWRITE_TAC [EL_GENLIST] \\
+    fs [LENGTH_GENLIST, valid_state_def])
+ \\ once_rewrite_tac [from_hardware_trans_def] \\ DEP_REWRITE_TAC [EL_GENLIST] \\
+    fs [valid_state_def, ORD_BOUND, valid_hardware_state_def, valid_hardware_trans_def] \\
+    first_x_assum (qspecl_then [`n2w s`, `n2w (ORD c)`] mp_tac) \\ simp [] \\
+    Cases_on `nos < dimword (:'a)` \\ fs [] \\ impl_tac
+    >- (fs [MOD_LESS, dimword_def] \\
+        qspecl_then [`dimindex (:'a)`, `s`] assume_tac bitTheory.MOD_2EXP_LT \\ simp [])
+    \\ simp []);
+
+val EL_from_hardware_trans = Q.store_thm("EL_from_hardware_trans",
+ `!nos c s trans.
+   valid_state nos s /\ valid_hardware_trans nos trans ==>
+   EL (w2n c) (EL s (from_hardware_trans nos trans)) = w2n (trans (n2w s) c)`,
+ rpt strip_tac \\ once_rewrite_tac [from_hardware_trans_def] \\
+ DEP_REWRITE_TAC [EL_GENLIST] \\ fs [valid_state_def] \\
+ Q.ISPEC_THEN `c` mp_tac w2n_lt \\ simp []);
+
+val EL_from_hardware_sif = Q.store_thm("EL_from_hardware_sif",
+ `!nos s sif. valid_state nos s ==> EL s (from_hardware_sif nos sif) = sif (n2w s)`,
+ rpt strip_tac \\ simp [from_hardware_sif_def] \\ `sif (n2w s) = (sif o n2w) s` by simp [] \\
+ pop_assum (fn th => PURE_REWRITE_TAC [th]) \\ match_mp_tac EL_GENLIST \\ fs [valid_state_def]);
+
+val ORD_CHR_w2n_8 = Q.store_thm("ORD_CHR_w2n_8",
+ `!(w:word8). ORD (CHR (w2n w)) = w2n w`,
+ gen_tac \\ Q.ISPEC_THEN `w` mp_tac w2n_lt \\ simp [ORD_CHR]);
+
+(****
+ circuit correctness
+ ****)
+
+val circuit_constants = Q.store_thm("circuit_constants",
+ `!n init ext.
+  (circuit init ext n).state_start = init.state_start /\
+  (circuit init ext n).state_is_final = init.state_is_final /\
+  (circuit init ext n).next_state_info = init.next_state_info`,
+ Induct \\ rw [circuit_def, regexp_def]);
+
+val circuit_accept_correct = Q.store_thm("circuit_accept_correct",
+ `!init ext state n.
+   (circuit init ext (SUC n)).accept = init.state_is_final (circuit init ext (SUC n)).state`,
+ ntac 3 gen_tac \\ Induct >- rw [circuit_def, regexp_def] \\
+ once_rewrite_tac [circuit_def] \\ simp [regexp_alt, circuit_constants]);
+
+(* TODO: Cleanup proof... *)
+(* NOTE: Maybe want to say something about accept for each cycle instead, i.e. construct the string by
+         searching backwards in time to previous new_package or beginning of time instead; in the end it
+         depends on what users of the circuit need I guess... *)
+val circuit_correct = Q.store_thm("circuit_correct",
+ `!nos init ext m n.
+   valid_hardware_state nos init.state /\
+   valid_hardware_state nos init.state_start /\
+   valid_hardware_trans nos init.next_state_info /\
+   (ext n).new_package ==>
+    (!p. p <= m ==> ~(ext (n + p)).new_package) ==>
+     (case exec_dfa_state (from_hardware_sif nos init.state_is_final)
+                          (from_hardware_trans nos init.next_state_info)
+                          (w2n init.state_start)
+                          (str_of_ext ext (n + 1) m) of (accept, state) =>
+      (circuit init ext (SUC (n + m))).accept = accept /\
+      (circuit init ext (SUC (n + m))).state = n2w state)`,
+ rpt strip_tac \\ Induct_on `m` >- simp [] \\ rpt strip_tac \\ TOP_CASE_TAC \\
+ qpat_x_assum `_ ==> _` mp_tac \\ impl_tac >- simp [] \\ TOP_CASE_TAC \\ strip_tac \\
+ once_rewrite_tac [circuit_def] \\ simp [regexp_alt, circuit_constants] \\
+ IF_CASES_TAC
+
+ (* new data *)
+ >- (simp [] \\ PURE_REWRITE_TAC [GSYM ADD_SUC] \\
+ qabbrev_tac `s = circuit init ext (SUC (n + m))` \\
+ qspecl_then [`ext`, `n + 1`, `m`] mp_tac str_of_ext_valid_data \\ impl_tac >- fs [ADD1] \\
+ strip_tac \\ fs [] \\ drule exec_dfa_state_APPEND \\
+ disch_then (qspec_then `STRING (CHR (w2n (ext (m + (n + 1))).data)) ""` mp_tac) \\
+ rewrite_tac [exec_dfa_state_def, ORD_CHR_w2n_8] \\ strip_tac \\ fs [] \\ rveq \\
+
+ DEP_REWRITE_TAC [EL_from_hardware_trans] \\ CONJ_TAC
+ >- metis_tac [exec_dfa_state_correct_valid_state,
+               valid_hardware_state_valid_state_w2n,
+               valid_hardware_trans_valid_trans]
+ >- (DEP_REWRITE_TAC [EL_from_hardware_sif] \\ simp [ADD1] \\
+    metis_tac [valid_hardware_state_valid_state_w2n,
+               valid_hardware_state_trans,
+               valid_state_valid_hardware_state,
+               exec_dfa_state_correct_valid_state,
+               valid_hardware_state_valid_state_w2n,
+               valid_hardware_trans_valid_trans]))
+
+ (* no new data, rewrite as above *)
+ \\ qsuff_tac `str_of_ext ext (n + 1) (SUC m) = str_of_ext ext (n + 1) m`
+  >- (strip_tac \\ fs [ADD_SUC] \\ rveq \\ fs [GSYM ADD_SUC, circuit_accept_correct])
+  \\ match_mp_tac str_of_ext_not_valid_data \\ fs [ADD1]);
+
+val circuit_correct_clean = Q.store_thm("circuit_correct_clean",
+ `!nos init ext m n.
+   valid_hardware_state nos init.state /\
+   valid_hardware_state nos init.state_start /\
+   valid_hardware_trans nos init.next_state_info /\
+   (ext n).new_package /\
+   (!p. p <= m ==> ~(ext (n + p)).new_package) ==>
+   (circuit init ext (SUC (n + m))).accept =
+   exec_dfa (from_hfinals (from_hardware_sif nos init.state_is_final))
+            (from_htable (from_hardware_trans nos init.next_state_info))
+            (w2n init.state_start)
+            (str_of_ext ext (n + 1) m)`,
+ rpt strip_tac \\ drule circuit_correct \\ rpt (disch_then drule) \\
+ TOP_CASE_TAC \\ DEP_REWRITE_TAC [GSYM exec_dfa_state_correct] \\
+ simp [] \\ metis_tac [valid_hardware_trans_valid_trans, valid_hardware_state_valid_state_w2n]);
+
+val lt_step = Q.prove(
+ `!P n m. (n < m <=> P) ==> (n < SUC m <=> (P \/ n = m))`,
+ rw [] \\ DECIDE_TAC);
+
+val lt_base = Q.prove(`n < 1 <=> n = 0`, DECIDE_TAC);
+
+val lt_256 = funpow (256 - 1) (MATCH_MP lt_step) lt_base |> EVAL_RULE;
+val lt_states = funpow (7 - 1) (MATCH_MP lt_step) lt_base |> EVAL_RULE; (* <-- TODO: hardcoded *)
+
+(* Slow but works *)
+val valid_hardware_trans_hwtable = prove(
+ ``valid_hardware_trans hwnos hwtable`` |> inst [ alpha |-> state_size_ty ],
+ rw [valid_hardware_trans_def, valid_hardware_state_def, hwnos_def, hwtable_def] \\
+ Cases_on `s` \\ fs [] \\ Cases_on `c` \\ fs [] \\
+
+ FULL_SIMP_TAC bool_ss [lt_states] \\ simp [] \\
+ FULL_SIMP_TAC bool_ss [lt_256] \\ EVAL_TAC);
+
+val INIT_def = Define `
+ INIT s <=>
+  s.state = 0w /\
+  s.state_start = 0w /\
+  s.state_is_final = hwfinal /\
+  s.next_state_info = hwtable`;
+
+(*local
+ val ss = wordsSyntax.mk_wordii (#start regexp_res, state_size)
+in
+val circuit_correct_clean' = 
+ circuit_correct_clean
+ |> Q.SPEC `hwnos`
+ |> Q.SPEC `<| state := ^ss; state_start := ^ss;
+               state_is_final := hwfinal;
+               next_state_info := hwtable |>`
+ |> SIMP_RULE (srw_ss()) [valid_hardware_trans_hwtable]
+ |> SIMP_RULE (srw_ss()) [valid_hardware_state_def, hwnos_def]
+ |> SPEC_ALL
+end;*)
+
+val circuit_correct_clean' = Q.prove(
+ `INIT s /\
+  (ext n).new_package ∧
+  (∀p. p ≤ m ⇒ ¬(ext (n + p)).new_package) ⇒
+  ((circuit s ext (SUC (n + m))).accept ⇔
+   exec_dfa (from_hfinals (from_hardware_sif hwnos hwfinal))
+            (from_htable (from_hardware_trans hwnos hwtable)) 0
+            (str_of_ext ext (n + 1) m))`,
+ rw [INIT_def] \\
+ qspecl_then [`hwnos`, `s`, `ext`, `m`, `n`] mp_tac circuit_correct_clean \\ impl_tac
+ >- (simp [valid_hardware_trans_hwtable] \\ simp [valid_hardware_state_def, hwnos_def])
+ \\ simp []);
+
+(* Evaluate final + table *)
+val circuit_correct_clean'' =
+ circuit_correct_clean'
+ |> CONV_RULE (RAND_CONV (RHS_CONV (RATOR_CONV (RATOR_CONV ((RAND_CONV EVAL) THENC (RATOR_CONV (RAND_CONV EVAL)))))));
+
+(* Evaluate table *)
+val cert' = 
+ cert
+ |> CONV_RULE (STRIP_QUANT_CONV (LHS_CONV (RATOR_CONV (RATOR_CONV (RAND_CONV EVAL)))));
+
+val circuit_correct_regexp = save_thm("circuit_correct_regexp",
+ circuit_correct_clean'' |> REWRITE_RULE [cert'] |> GEN_ALL);
+
+val _ = export_theory ();
