translator/verilogPrintScript.sml
@@ -4,24 +4,34 @@ open verilogTheory;
 
 val _ = new_theory "verilogPrint";
 
-val buop_print = Define `
+val buop_print_def = Define `
  buop_print Not = "!"`;
 
-val bbop_print = Define `
+val bbop_print_def = Define `
  (bbop_print And = "&&") /\
  (bbop_print Equal = "==") /\
  (bbop_print NotEqual = "!=") /\
  (bbop_print Or = "||")`;
 
-val abop_print = Define `
+val abop_print_def = Define `
  (abop_print BitwiseAnd = "&") /\
  (abop_print BitwiseOr = "|") /\
  (abop_print BitwiseXor = "^^")`;
 
-val arith_print = Define `
+val arith_print_def = Define `
  (arith_print Minus = "-") /\
  (arith_print Plus = "+") /\
  (arith_print Times = "*") /\
  (arith_print Mod = "%")`;
+
+val type_print_idx_def = Define `
+ type_print_idx i = "[" ++ toString (i - 1) ++ ":0]"`;
+
+val type_print_def = Define `
+ (type_print VBool_t = "logic") /\
+ (type_print (VArray_t is) = "logic" ++ CONCAT (MAP type_print_idx is))`;
+
+val var_type_print_def = Define `
+ var_type_print xs = MAP (\(var, ty). type_print ty ++ " " ++ var) xs`;
 
 val _ = export_theory ();
